Add GetContext effect to eio case study.

theories/case_studies/eio/eio.v
@@ -2,6 +2,7 @@
 
 (* a.d. TODO do we really need the saved proposition. Check again if the lookup lemma can be proven without it.
 If not, write an explanation why. *)
+(* a.d. TODO clean up + convert everything to camelCase. *)
 
 (* a.d. TODO rewrite
    The ability offered by effect handlers (or any other interface for
@@ -35,11 +36,13 @@ From case_studies.eio Require Import atomics concurrent_queue cqs.
 (* ========================================================================== *)
 (** * Implementation of the Scheduler. *)
 
-Notation Fork e := (InjL e) (only parsing).
-Notation Suspend f := (InjR f) (only parsing).
+Notation Fork state e := (InjL (Pair state e)) (only parsing).
+Notation Suspend f := (InjR (InjL f)) (only parsing).
+Notation GetContext := (InjR (InjR #())) (only parsing).
 
-Notation Fork' e := (InjLV e) (only parsing).
-Notation Suspend' f := (InjRV f) (only parsing).
+Notation Fork' state e := (InjLV (PairV state e)) (only parsing).
+Notation Suspend' f := (InjRV (InjLV f)) (only parsing).
+Notation GetContext' := (InjRV (InjRV #())) (only parsing).
 
 Notation Done y := (InjL y) (only parsing).
 Notation Waiting ws := (InjR ws) (only parsing).
@@ -53,8 +56,13 @@ Section implementation.
   Definition new_promise : val := (λ: <>,
     ref (Waiting (cqs_new #()))
   )%V.
-  Definition fork : val := (λ: "f", do: (Fork "f"))%V.
+  Definition new_fiber_state : val := (λ: <>,
+    ref #0
+  )%V.
+  Definition fork : val := (λ: "state" "f", do: (Fork "state" "f"))%V.
   Definition suspend : val := (λ: "f", do: (Suspend "f"))%V.
+  Definition get_context : val := (λ: <>, do: GetContext)%V.
+
   Definition next : val := (λ: "q",
     match: queue_pop "q" with
       (* Empty *) InjL <> => #()
@@ -74,9 +82,10 @@ Section implementation.
 
   (* fork a new fiber "f" and return a promise to get the result. *)
   Definition fork_promise : val := (λ: "f", 
+    let: "state" := get_context #() in
     let: "p" := new_promise #() in
     let: "wrapped_f" := fork_wrap_f "f" "p" in
-    fork "wrapped_f";;
+    fork "state" "wrapped_f";;
     "p")%V.
    
   Definition await_callback : val := (λ: "p" "ws", (λ: "waker", 
@@ -112,28 +121,36 @@ Section implementation.
         end
     end
   )%V.
-
+    
   Definition run : val := (λ: "main",
+    let: "initial_state" := new_fiber_state #() in
     let: "q" := queue_create #() in
-    let: "fulfill" := rec: "fulfill" "e" :=
-      deep-try: "e" #() with
+    let: "fulfill" := rec: "fulfill" "state" "f" :=
+      deep-try: "f" #() with
         effect (λ: "request" "k",
           match: "request" with
-            (* Fork: *) InjL "e" =>
+            (* Fork: *) InjL "statef" =>
+              let: "fork_state" := Fst "statef" in
+              let: "fork_f" := Snd "statef" in
               queue_push "q" (λ: <>, "k" #());;
-              "fulfill" "e"
-          | (* Suspend: *) InjR "suspender" =>
-              (* a.d. probably the most complicated line 
-              When waker is called with a value v, a closure calling the continuation with v is put into the run_queue. 
-              suspender can either put waker somewhere that causes it to be called later or just call it directly. *)
-              let: "waker" := (λ: "v", queue_push "q" (λ: <>, "k" "v")) in
-              "suspender" "waker";;
-              next "q"
+              "fulfill" "fork_state" "fork_f"
+          | (* Suspend/GetContext: *) InjR "e1" =>
+            match: "e1" with
+              (* Suspend: *) InjL "suspender" =>
+                (* a.d. probably the most complicated line 
+                When waker is called with a value v, a closure calling the continuation with v is put into the run_queue. 
+                suspender can either put waker somewhere that causes it to be called later or just call it directly. *)
+                let: "waker" := (λ: "v", queue_push "q" (λ: <>, "k" "v")) in
+                "suspender" "waker";;
+                next "q"
+            | (* GetContext: *) InjR <> =>
+                "k" "state"
+            end
           end)
       | return (λ: <>, next "q")
       end
     in
-    "fulfill" "main"
+    "fulfill" "initial_state" "main"
   )%V.
 
 End implementation.
@@ -165,19 +182,25 @@ End implementation.
    indeed unreachable: if a fiber cannot find its own promise fulfilled by
    another fiber, then its token has been duplicated, which situation is
    contradictory. *)
-   
+
 (* The assumption that certain cameras are available. *)
 Class promiseGpreS Σ := {
   promise_mapG :> inG Σ
     (authR (gmapUR (loc * gname * gname) unitR));
+  (* state_mapG :> inG Σ
+    (authR (gmapUR gname (agreeR locO))); *)
   torchG :> inG Σ (csumR fracR (agreeR unitO));
+  stateG :> inG Σ (agreeR locO);
 }.
   
 (* A concrete instance of [Σ] for which the assumption [promisesGS Σ] holds. *)
 Definition promiseΣ := #[
   GFunctor (authRF
     (gmapURF (loc * gname * gname) unitR));
-  GFunctor (csumR fracR (agreeR unitO))
+  (* GFunctor (authRF
+    (gmapURF gname (agreeR locO))); *)
+  GFunctor (csumR fracR (agreeR unitO));
+  GFunctor (agreeR locO)
 ].
   
 (* The proof of the previous claim. *)
@@ -203,7 +226,20 @@ Section predicates.
   Definition promise_state_whole γ := own γ (Cinl 1%Qp).
   Definition promise_state_waiting γ := own γ (Cinl (1/2)%Qp).
   Definition promise_state_done γ := own γ (Cinr (to_agree ())).
+  
+  (* a.d. TODO I wonder if we can reformulate isMember so that we don't even need isState.
+     We need it so that we have a single gname γ to identify each thread for use in the GetContext effect.
+     *)
+  Definition isFiberState δ (l: loc): iProp Σ :=
+    own δ (to_agree l).
+    
+  Definition fiberState δ (l : loc) : iProp Σ := 
+    (isFiberState δ l ∗ ∃ (n:nat), l ↦ #n)%I.
 
+  (* This resource is always held by the active fiber, so we need to pass it in and out of effects 
+     and need it as a precondition of a ready fiber. *)
+  Definition fiberContext δ := (∃ (l : loc), fiberState δ l)%I.
+    
   (* Fragment of the promise map. *)
   Definition isMember p γ ε :=
     own promise_name (◯ {[(p, γ, ε) := tt]}).
@@ -251,8 +287,8 @@ Section predicates.
         Using saved_pred we can get look up one promise in the promise map and then get a (▷ Φ y) 
      If waiting, then there exists a cqs that contains wakers. *)
   Definition promiseInv_inner : iProp Σ := (
-    ∃ M, isPromiseMap M ∗ 
-      [∗ map] args ↦ tt ∈ M, let '(p, γ, ε) := args in
+    ∃ M, isPromiseMap M ∗
+      ([∗ map] args ↦ tt ∈ M, let '(p, γ, ε) := args in
         ((* Fulfilled: *) ∃ y,
           p ↦ Done' y ∗ promise_state_done γ ∗ 
           ∃ (Φ: val -d> iPropO Σ), isPromiseResult ε Φ ∗ □ Φ y)
@@ -262,7 +298,7 @@ Section predicates.
           promise_state_waiting γ ∗
           (∃ n, thread_queue_state n) ∗
           resume_all_permit ∗
-          promise_cqs wakers)
+          promise_cqs wakers))
   )%I.
     
   Definition promiseInv := inv promiseN promiseInv_inner.
@@ -272,8 +308,8 @@ Section predicates.
 
   (* Now ready is just a predicate on a continuation k, that k is safe to execute under the assumption
      that promiseInv holds. *)
-  Definition ready (k: val) : iProp Σ := (
-    promiseInv -∗ EWP (k #()) {{ _, True }}
+  Definition ready (δ : gname) (k: val) : iProp Σ := (
+    fiberContext δ -∗ promiseInv -∗ EWP (k #()) {{ _, True }}
   )%I.
 
   Definition promiseSt p γ ε: iProp Σ :=
@@ -287,7 +323,7 @@ Section predicates.
       (∃ n, thread_queue_state n) ∗
       resume_all_permit ∗
       promise_cqs wakers).
-
+      
   Definition promiseSt_later p γ ε : iProp Σ :=
     ((* Fulfilled: *) ∃ y,
        p ↦ Done' y ∗ promise_state_done γ ∗
@@ -303,22 +339,24 @@ Section predicates.
   (* ------------------------------------------------------------------------ *)
   (* Non-expansiveness. *)
 
+  (* a.d. TODO we don't need it anymore since ready is not recursive, but it should still hold with the new formulation.
+      It broke after I added the δ argument. *)
   (* [ready]. *)
-  Global Instance ready_ne n :
-    Proper ((dist n) ==> (dist n)) ready.
+  (* Global Instance ready_ne δ n :
+    Proper ((dist n) ==> (dist n) ==> (dist n)) ready.
   Proof.
     induction (lt_wf n) as [n _ IH]=>k k' ->.
     rewrite /ready.
-    by repeat (f_contractive
+    (* by repeat (f_contractive
            || f_equiv || apply IH 
            || case x1 as ()         || case x2 as ()
            || case y1 as (y11, y12) || case y2 as (y21, y22)
-           || apply H0 || apply H1 ).
-  Qed.
-  Global Instance ready_proper : Proper ((≡) ==> (≡)) ready.
-  Proof. intros ???. apply equiv_dist=>n.
-         by apply ready_ne; apply equiv_dist.
-  Qed.
+           || apply H0 || apply H1 ). *)
+  Admitted.
+  Global Instance ready_proper : Proper ((≡) ==> (≡) ==> (≡)) ready.
+  (* Proof. intros ???. apply equiv_dist=>n.
+         by apply ready_ne; apply equiv_dist. *)
+  Admitted. *)
 
 
   (* ------------------------------------------------------------------------ *)
@@ -376,6 +414,39 @@ Section predicates.
     Qed.
 
   End promise_state.
+  
+  Section fiber_state.
+    Global Instance isFiberState_persistent δ l: Persistent (isFiberState δ l).
+    Proof. by apply _. Qed.
+
+    Lemma fiber_state_create (l: loc) : ⊢ |==> ∃ δ, isFiberState δ l.
+    Proof. by iMod (own_alloc (to_agree l)) as (δ) "Hfs"; last iExists δ. Qed.
+    
+    Lemma is_fiber_state_agree (l l' : loc) δ : 
+      isFiberState δ l -∗ isFiberState δ l' -∗ ⌜ l = l' ⌝.
+    Proof.
+      iIntros "H H'". 
+      iCombine "H H'" as "H".
+      iPoseProof (own_valid with "H") as "%".
+      iPureIntro.
+      by apply to_agree_op_inv_L.
+    Qed.
+
+    Lemma fiber_state_agree (l l' : loc) δ : 
+      fiberState δ l -∗ isFiberState δ l' -∗ ⌜ l = l' ⌝ ∗ fiberState δ l.
+    Proof.
+      iIntros "(#H & HRest) #H'". 
+      iSplitR; first by iApply is_fiber_state_agree.
+      by iFrame.
+    Qed.
+    
+    Lemma fiber_context_agree (l : loc) δ :
+      fiberContext δ -∗ isFiberState δ l -∗ fiberState δ l.
+    Proof.
+      iIntros "(% & HfState) H".
+      by iDestruct (fiber_state_agree with "HfState H") as (->) "HfState".
+    Qed.
+  End fiber_state.
 
   (* Logical rules governing the predicate [ready]. *)
   Section ready.
@@ -439,7 +510,7 @@ Section predicates.
         promiseInv_inner ∗ isMember p γ ε.
     Proof.
       iIntros "(HpInv & Hp)". rewrite /promiseInv_inner.
-      iDestruct "HpInv" as (M) "[HM HInv]".
+      iDestruct "HpInv" as (M) "(HM & HInv)".
       destruct (M !! (p, γ, ε)) as [Ψ|] eqn:Hlkp.
       - rewrite (big_opM_delete _ _ _ _ Hlkp).
         iDestruct "HInv" as "[Hp' _]".
@@ -497,59 +568,69 @@ End predicates.
 
 Section protocol_coop.
   Context `{!heapGS Σ, !promiseGS Σ, !savedPredG Σ val}.
+  
+  Notation pEff := (gnameO -d> iEffO) (only parsing).
+  
+  Definition FORK_pre (Coop : pEff) (δ : gname): iEff Σ :=
+    >> (ℓstate : loc) e >> !(Fork' #ℓstate e) {{fiberState δ ℓstate ∗ ▷ (fiberContext δ -∗ EWP e #() <|Coop δ |> {{_, fiberContext δ}}) }};
+    << (_: val) << ?(#())        {{ fiberState δ ℓstate }} @ OS.
 
-  Definition FORK_pre (Coop : iEff Σ) : iEff Σ :=
-    >> e >> !(Fork'  e) {{promiseInv ∗ ▷ (promiseInv -∗  EWP e #() <|Coop |> {{_, True}} ) }};
-    << (_: val) << ?(#())        {{ True }} @ OS.
-      
-  Definition SUSPEND : iEff Σ :=
+      (* a.d. TODO I think I can delete promiseInv from SUSPEND *)
+  Definition SUSPEND (δ : gname) : iEff Σ :=
     >> (f: val) (P: val → iProp Σ) >> !(Suspend' f) {{
       (* We call suspender with the waker function and waker receives a value satisfying P. *)
         ( (∀ (waker: val),
           (∀ (v: val), P v -∗  (EWP (waker v) <| ⊥ |> {{_, True }}) ) -∗
           promiseInv -∗ (▷ EWP (f waker) <| ⊥ |> {{_, True  }}) ) 
       ∗
-        promiseInv)%I
+        fiberContext δ ∗ promiseInv)%I
     }};
-    << y           << ?(y)         {{ P y }} @ OS.
+    << y           << ?(y)         {{ P y ∗ fiberContext δ }} @ OS.
 
-  Definition Coop_pre : (iEffO) → (iEffO) := (λ Coop,
-    FORK_pre Coop <+> SUSPEND
+  Definition GET_CONTEXT (δ: gname ): iEff Σ :=
+    >> (_: val) >> !(GetContext') {{ True }};
+    << (state : loc) << ?(#state) 
+        {{isFiberState δ state}} @ OS.
+
+  Definition Coop_pre : pEff → pEff := (λ Coop,
+    λ δ, FORK_pre Coop δ <+> SUSPEND δ <+> GET_CONTEXT δ
   )%ieff.
 
   Local Instance Coop_pre_contractive : Contractive (Coop_pre).
   Proof.
-    rewrite /Coop_pre /SUSPEND /FORK_pre=> n Coop Coop' HCoop.
+    intros n'.
+    rewrite /Coop_pre /SUSPEND /FORK_pre /GET_CONTEXT=> n Coop Coop' HCoop.
     by repeat (apply ewp_ne||apply iEffPre_base_ne||f_contractive||f_equiv).
   Qed.
-  Definition Coop_def : (iEff Σ) := fixpoint Coop_pre.
+  Definition Coop_def : (gname → iEff Σ) := fixpoint Coop_pre.
   Definition Coop_aux : seal Coop_def. Proof. by eexists. Qed.
   Definition Coop := Coop_aux.(unseal).
   Definition Coop_eq : Coop = Coop_def := Coop_aux.(seal_eq).
-  Global Lemma Coop_unfold  : Coop  ≡ Coop_pre (Coop).
+  Global Lemma Coop_unfold δ : Coop δ  ≡ Coop_pre Coop δ.
   Proof. rewrite Coop_eq /Coop_def.
          by apply (fixpoint_unfold (Coop_pre)).
   Qed.
   Definition FORK := FORK_pre Coop.
 
-  Lemma upcl_Coop v Φ' :
-    iEff_car (upcl OS (Coop )) v Φ' ⊣⊢
-      iEff_car (upcl OS (FORK )) v Φ' ∨
-      iEff_car (upcl OS (SUSPEND )) v Φ'.
+  Lemma upcl_Coop v Φ' δ:
+    iEff_car (upcl OS (Coop δ)) v Φ' ⊣⊢
+      iEff_car (upcl OS (FORK δ)) v Φ' ∨
+      iEff_car (upcl OS (SUSPEND δ)) v Φ' ∨
+      iEff_car (upcl OS (GET_CONTEXT δ)) v Φ'.
   Proof.
-    transitivity (iEff_car (upcl OS (Coop_pre Coop )) v Φ').
+    transitivity (iEff_car (upcl OS (Coop_pre Coop δ)) v Φ').
     - iApply iEff_car_proper. by rewrite {1}Coop_unfold.
-    - by rewrite upcl_sum (upcl_tele' [tele _ _] [tele _]) //.
+    - by rewrite upcl_sum upcl_sum (upcl_tele' [tele _ _] [tele _]) //.
   Qed.
 
-  Lemma upcl_FORK  v Φ' :
-    iEff_car (upcl OS (FORK )) v Φ' ≡
-      (∃ e, ⌜ v = Fork' e ⌝ ∗ (promiseInv ∗ ▷ (promiseInv -∗ EWP e #() <|Coop|> {{_, True }})) ∗
-            (∀ (_ : val), True -∗ Φ' #()))%I.
-  Proof. by rewrite /FORK (upcl_tele' [tele _] [tele _]). Qed.
+  Lemma upcl_FORK δ v Φ' :
+    iEff_car (upcl OS (FORK δ)) v Φ' ≡
+      (∃ (ℓstate: loc) e, ⌜ v = Fork' #ℓstate e ⌝ ∗ (fiberState δ ℓstate ∗ ▷ (fiberContext δ -∗ EWP e #() <|Coop δ|> {{_, fiberContext δ }})) ∗
+            (∀ (_ : val), fiberState δ ℓstate -∗ Φ' #()))%I.
+  Proof. by rewrite /FORK (upcl_tele' [tele _ _] [tele _]). Qed.
 
-  Lemma upcl_SUSPEND  v Φ' :
-    iEff_car (upcl OS (SUSPEND )) v Φ' ≡
+  Lemma upcl_SUSPEND δ v Φ' :
+    iEff_car (upcl OS (SUSPEND δ)) v Φ' ≡
       (∃ (f : val) (P: val → iProp Σ), ⌜ v = Suspend' f ⌝ 
       ∗ 
       (* the big precondition of the protocol *)
@@ -557,10 +638,17 @@ Section protocol_coop.
           (∀ (v: val), P v -∗ (EWP (waker v) <| ⊥ |> {{_, True }}) ) -∗
           promiseInv -∗ (▷ EWP (f waker) <| ⊥ |> {{_, True }}) )
       ∗
-          promiseInv) 
+          fiberContext δ ∗ promiseInv) 
       ∗
-          (∀ v, P v -∗ Φ' v))%I.
+          (∀ v, (P v ∗ fiberContext δ) -∗ Φ' v))%I.
   Proof. by rewrite /SUSPEND (upcl_tele' [tele _ _] [tele _]). Qed.
+
+  Lemma upcl_GET_CONTEXT δ v Φ' :
+    iEff_car (upcl OS (GET_CONTEXT δ)) v Φ' ≡ 
+      (∃ (_: val), ⌜ v = GetContext' ⌝ ∗ True ∗
+        (∀ (ℓstate : loc), isFiberState δ ℓstate -∗ Φ' #ℓstate)
+      )%I.
+  Proof. by rewrite /GET_CONTEXT (upcl_tele' [tele _] [tele _]). Qed.
 
 End protocol_coop.
 
@@ -602,12 +690,22 @@ Section verification.
     iExists p, γ, ε. iFrame. by auto.
   Qed.
   
-  Lemma ewp_next q Ψ :
+  Lemma ewp_new_fiber_state :
+    ⊢ EWP new_fiber_state #() {{ state, ∃ (ℓstate : loc) (n: nat), ⌜ state = #ℓstate ⌝ ∗ ℓstate ↦ #n }}.
+  Proof.
+    iIntros. rewrite /new_fiber_state.
+    ewp_pure_steps. iApply ewp_alloc.
+    iIntros "!>" (ℓstate) "Hstate !>".
+    iExists _, 0. by iFrame. 
+  Qed.
+    
+  Lemma ewp_next δ q Ψ :
+    fiberContext δ -∗
     promiseInv -∗
-      is_queue q ready -∗
+      is_queue q (ready δ) -∗
          EWP (next q) <| Ψ |> {{ _, True }}.
   Proof.
-    iIntros "HpInv #Hq". unfold next. ewp_pure_steps. ewp_bind_rule.
+    iIntros "HfCtx HpInv #Hq". unfold next. ewp_pure_steps. ewp_bind_rule.
     iApply ewp_mono; [iApply (queue_pop_spec with "Hq")|].
     simpl. iIntros (y) "[->|(%k & -> & Hk)] !>".
     - (* queue is empty *) 
@@ -615,35 +713,44 @@ Section verification.
     - (* queue has a continuation *)
       ewp_pure_steps.
       rewrite /ready.
-      iSpecialize ("Hk" with "HpInv").
+      iSpecialize ("Hk" with "HfCtx HpInv").
       iApply ewp_os_prot_mono. { by iApply iEff_le_bottom. } { done. }
   Qed.
 
-  Lemma ewp_fork (e : val) :
-    promiseInv  ∗ 
-    (promiseInv -∗ EWP e #() <| Coop |> {{ _, True }})
+  Lemma ewp_fork (ℓstate : loc) (e : val) δ :
+    fiberState δ ℓstate ∗ (fiberContext δ -∗ EWP e #() <| Coop δ|> {{ _, fiberContext δ }})
   ⊢
-      EWP (fork e) <| Coop |> {{ _, True }}.
+      EWP (fork #ℓstate e) <| Coop δ |> {{ _, fiberState δ ℓstate }}.
   Proof.
-    iIntros "(HpInv &  He)". rewrite /fork. ewp_pure_steps.
+    iIntros "(Hfstate & He)". rewrite /fork. ewp_pure_steps.
     iApply ewp_do_os. rewrite upcl_Coop upcl_FORK. iLeft.
-    iExists e. iSplit; [done|]. iFrame.
-    iIntros (_) "H". by iFrame.
+    iExists ℓstate, e. iSplit; [done|]. iFrame.
+    iIntros (_) "H". by done.
   Qed.
 
-  Lemma ewp_suspend (f : val) (P: val → iProp Σ) :
+  Lemma ewp_suspend (f : val) (P: val → iProp Σ) δ :
       ( (∀ (waker: val),
         (∀ (v: val), P v -∗ (EWP (waker v) <| ⊥ |> {{_, True}}) ) -∗
         promiseInv -∗ (▷ EWP (f waker) <| ⊥ |> {{_, True }})) 
     ∗
-      promiseInv) 
+      fiberContext δ ∗ promiseInv) 
     ⊢
-      EWP (suspend f) <| Coop |> {{ v, P v }}.
+      EWP (suspend f) <| Coop δ |> {{ v, P v ∗ fiberContext δ }}.
   Proof.
     iIntros "(He & HpInv)". rewrite /suspend. ewp_pure_steps.
-    iApply ewp_do_os. rewrite upcl_Coop upcl_SUSPEND. iRight.
+    iApply ewp_do_os. rewrite upcl_Coop upcl_SUSPEND. iRight; iLeft.
     iExists f, P. iSplit; [done|]. iFrame.
     iIntros (v) "Hv". by iFrame.
+  Qed.
+  
+  Lemma ewp_get_context δ : 
+    ⊢ EWP (get_context #()) <| Coop δ |> {{ state, ∃ (ℓstate: loc), ⌜ state = #ℓstate ⌝ ∗ isFiberState δ ℓstate }}.
+  Proof.
+    iIntros. rewrite /get_context. ewp_pure_steps.
+    iApply ewp_do_os. rewrite upcl_Coop upcl_GET_CONTEXT. iRight; iRight.
+    iExists #(). iSplit; [done|]. iSplit; [done|].
+    iIntros (?) "H". iExists ℓstate. iSplit; first done.
+    done.
   Qed.
   
   Lemma ewp_await_callback (p: loc) (wakers: val) γ ε Φ:
@@ -711,11 +818,11 @@ Section verification.
       + ewp_pure_steps. by done.
   Qed.
   
-  Lemma ewp_await (p: loc) Φ :
-    promiseInv ∗ isPromise p Φ ⊢ 
-      EWP (await #p) <| Coop |> {{v, □ Φ v}}.
+  Lemma ewp_await (p: loc) Φ δ :
+    fiberContext δ ∗ promiseInv ∗ isPromise p Φ ⊢ 
+      EWP (await #p) <| Coop δ |> {{v, □ Φ v ∗ fiberContext δ}}.
   Proof.
-    iIntros "(#HpInv & %γ & %ε & #Hmem & #Hε)". rewrite /await. 
+    iIntros "(HfCtx & #HpInv & %γ & %ε & #Hmem & #Hε)". rewrite /await. 
     ewp_pure_steps. ewp_bind_rule. simpl.
     (* a.d. here we need to open the invariant to read the promise *)
     rewrite /promiseInv.
@@ -731,11 +838,11 @@ Section verification.
       iApply (fupd_trans_frame (⊤ ∖ ↑promiseN) (⊤ ∖ ↑promiseN) ⊤ _ (▷ promiseInv_inner)).
       iSplitL "Hclose". iApply "Hclose".
       iModIntro.
-      iSplitL.
+      iSplitR "HfCtx".
       iNext. iApply "HpInvIn". iLeft. iExists y. iFrame. iSplit; first by done.
       iExists Φ'. by iSplit.
       ewp_pure_steps. 
-      iModIntro.
+      iFrame. iModIntro.
       by iRewrite "Heqv".
     - (* the promise is not yet fulfilled, so we create a callback and perform the suspend effect.
          After the suspend returns, we know the promise is fulfilled. *)
@@ -747,7 +854,7 @@ Section verification.
       iApply (fupd_trans_frame (⊤ ∖ ↑promiseN) (⊤ ∖ ↑promiseN) ⊤ _ (▷ promiseInv_inner)).
       iSplitL "Hclose". iApply "Hclose".
       iModIntro.
-      iSplitR "HIsSus".
+      iSplitR "HIsSus HfCtx".
       iNext. iApply "HpInvIn". iRight. iExists wakers. iFrame.
       iSplit; last done. by iExists (S n). 
       ewp_pure_steps. 
@@ -761,11 +868,11 @@ Section verification.
       iIntros (callback) "Hf !>".
       ewp_pure_steps.
       ewp_bind_rule. simpl.
-      iApply (ewp_mono with "[Hf]").
+      iApply (ewp_mono with "[Hf HfCtx]").
       { iApply (ewp_suspend callback (λ v, ⌜ v = #() ⌝ ∗ promise_state_done γ)%I). 
         by iFrame. }
       (* after we have performed the effect we get promise_state_done. *)
-      iIntros (v) "(-> & Hps) !>".
+      iIntros (v) "((-> & Hps) & HfCtx) !>".
       ewp_pure_steps. ewp_bind_rule. simpl.
       (* now we match on the promise again but this time we know it must be fulfilled *)
       iClear "Hwakers". clear wakers.
@@ -781,29 +888,31 @@ Section verification.
       iApply (fupd_trans_frame (⊤ ∖ ↑promiseN) (⊤ ∖ ↑promiseN) ⊤ _ (▷ promiseInv_inner)).
       iSplitL "Hclose". iApply "Hclose".
       iModIntro.
-      iSplitL.
+      iSplitR "HfCtx".
       iNext. iApply "HpInvIn". iLeft. iExists y. iFrame. 
       iExists Φ'. by iSplit.
       ewp_pure_steps.
+      iFrame.
       by iRewrite "Heqv".
   Qed.
 
   (* the wrapped function is passed via the FORK effect to the handler.
      the handler should then pass is_queue to wrapped_f so that it is able to change the run_queue.
      is_queue should be passed between client and handler the same as promiseInv, for every performed effect. *)
-  Lemma ewp_fork_wrap (f: val) (p: loc) γ ε Φ :
-    promise_state_waiting γ ∗ isMember p γ ε ∗ isPromiseResult ε Φ ∗ EWP (f #()) <| Coop |> {{v, □ Φ v}} 
+  Lemma ewp_fork_wrap (f: val) (p: loc) γ δ ε Φ :
+    promise_state_waiting γ ∗ isMember p γ ε ∗ isPromiseResult ε Φ ∗ (fiberContext δ -∗ EWP (f #()) <| Coop δ |> {{v, □ Φ v ∗ fiberContext δ}}) 
   ⊢
     EWP (fork_wrap_f f #p) <| ⊥ |> {{wrapped_f, 
         (* promiseInv and is_queue are passed here because they come from the effect handler *)
           promiseInv -∗
-          EWP (wrapped_f #()) <| Coop |> {{_, True}} }}.
+          fiberContext δ -∗ EWP (wrapped_f #()) <| Coop δ |> {{_, fiberContext δ }} }}.
   Proof.
     iIntros "(Hps_start & #Hmem & #Hε & Hf)". 
     rewrite /fork_wrap_f. ewp_pure_steps.
-    iIntros "#HpInv". ewp_pure_steps.
+    iIntros "#HpInv HfCtx". ewp_pure_steps.
+    iSpecialize ("Hf" with "HfCtx").
     ewp_bind_rule. simpl. iApply (ewp_mono with "Hf"). 
-    iIntros (v) "#Hv !>".
+    iIntros (v) "(#Hv & HfCtx) !>".
     ewp_pure_steps. ewp_bind_rule. simpl.
     (* a.d. here we need to open the invariant *)
     rewrite /promiseInv.
@@ -819,7 +928,7 @@ Section verification.
     iApply (fupd_trans_frame (⊤ ∖ ↑promiseN) (⊤ ∖ ↑promiseN) ⊤ _ (▷ promiseInv_inner)).
     iSplitL "Hclose". iApply "Hclose".
     iModIntro.
-    iSplitR "Hps_start".
+    iSplitR "Hps_start HfCtx".
     iNext. iApply "HpInvIn". iRight. iExists wakers. by iFrame.
     ewp_pure_steps. ewp_bind_rule. simpl.
     (* now we change the logical promise state, but for that we need to open it again. *)
@@ -835,7 +944,7 @@ Section verification.
     iApply (fupd_trans_frame (⊤ ∖ ↑promiseN) (⊤ ∖ ↑promiseN) ⊤ _ (▷ promiseInv_inner)).
     iSplitL "Hclose". iApply "Hclose".
     iModIntro.
-    iSplitR "Htqstate Hres".
+    iSplitR "Htqstate Hres HfCtx".
     iNext. iApply "HpInvIn". iLeft. iExists v. iFrame. iSplit; first done.
     iExists Φ. by iSplit.
     ewp_pure_steps. ewp_bind_rule. simpl.
@@ -848,74 +957,106 @@ Section verification.
     iIntros (?) "_ !>". by done.
   Qed.
 
-  Lemma ewp_fork_promise  (f: val) Φ :
-    promiseInv ∗ EWP (f #()) <| Coop  |> {{v, □ Φ v}}
+  Lemma ewp_fork_promise (f: val) Φ δ :
+    fiberContext δ ∗ promiseInv ∗ (fiberContext δ -∗ EWP (f #()) <| Coop δ |> {{v, □ Φ v ∗ fiberContext δ}})
   ⊢ 
-    EWP (fork_promise f) <| Coop  |> {{ y, 
-      ∃ (p: loc), ⌜ y = #p ⌝ ∗ isPromise p Φ }}.
+    EWP (fork_promise f) <| Coop δ |> {{ y, 
+      ∃ (p: loc), ⌜ y = #p ⌝ ∗ isPromise p Φ ∗ fiberContext δ }}.
   Proof.
-    iIntros "(#HpInv & Hf)". rewrite /fork_promise. ewp_pure_steps.
+    iIntros "(HfCtx & #HpInv & Hf)". rewrite /fork_promise. ewp_pure_steps.
+    ewp_bind_rule. simpl.
+    iApply ewp_mono.
+    iApply ewp_get_context.
+    iIntros (state) "(%ℓstate & -> & #HIsState) !>".
+    ewp_pure_steps.
     ewp_bind_rule. simpl.
     iApply ewp_mono. 
     iApply ewp_os_prot_mono. 
       by iApply iEff_le_bottom. 
     iApply (ewp_new_promise Φ with "HpInv").
-    iIntros (v) "(%p & %γ & %ε & -> & Hps & #Hmem) !>".
+    iIntros (v) "(%p & %γ & %ε & -> & Hps & #(Hmem & HRes)) !>".
     ewp_pure_steps.
     iApply (ewp_bind' (AppRCtx _)); first done. simpl.
     iApply (ewp_mono with "[Hf Hps]").
     { iApply ewp_os_prot_mono. iApply iEff_le_bottom.
-      iApply ewp_fork_wrap. by iFrame. }
+      iApply ewp_fork_wrap. iFrame. by iSplit. }
     iIntros (wrapped_f) "Hwrapped_f !>".
+    iSpecialize ("Hwrapped_f" with "HpInv").
     ewp_pure_steps.
-    ewp_bind_rule. simpl.
-    iApply (ewp_mono with "[HpInv Hwrapped_f]").
-    iApply ewp_fork. by iFrame.
-    iIntros (?) "_ !>".
+    iApply (ewp_bind' (AppRCtx _)); first done. simpl.
+    iApply (ewp_mono with "[Hwrapped_f HfCtx]").
+    iApply ewp_fork. 
+    iPoseProof (fiber_context_agree with "HfCtx HIsState") as "HfState".
+    by iFrame.
+    iIntros (?) "HfState !>".
     ewp_pure_steps. iExists p.
     iFrame. iSplit; first done.
-    by iExists γ, ε.
+    iSplitR.
+    iExists γ, ε. by iSplit.
+    by iExists _.
   Qed.
       
   Lemma ewp_run (main : val) Φ :
-    promiseInv ∗ EWP main #() <| Coop |> {{ v, □ Φ v }} ⊢
+    promiseInv ∗ (∀ δ, fiberContext δ -∗ EWP main #() <| Coop δ |> {{ v, □ Φ v ∗ fiberContext δ }}) ⊢
       EWP run main {{ _, True }}.
   Proof.
     iIntros "(#HpInv & Hmain)". unfold run. ewp_pure_steps.
-    ewp_bind_rule. iApply ewp_mono. { by iApply queue_create_spec. }
-    iIntros (q) "Hq !>". simpl. ewp_pure_steps.
-    iSpecialize ("Hq" $! ready).
-    iLöb as "IH" forall (main q Φ).
+    ewp_bind_rule. simpl. iApply ewp_mono. { by iApply ewp_new_fiber_state. }
+    iIntros (state) "H".
+    iDestruct "H" as (ℓstate n) "(-> & Hℓstate)".
+    iMod (fiber_state_create ℓstate) as (δ) "#HIsState".
+    (* a.d. We must do this up here so that ∀ δ does not appear in IH.
+       a.d. TODO can we speciaize Hℓstate, too? *)
+    iSpecialize ("Hmain" $! δ).
+    iModIntro. ewp_pure_steps.
+    ewp_bind_rule. simpl. iApply ewp_mono. { by iApply queue_create_spec. }
+    iIntros (q) "Hq !>". 
+    (* a.d. it's kind of interesting that ready is now also scheduler specific. But it's nice to know that
+       we cannot schedule a fiber in a different scheduler. *)
+    iSpecialize ("Hq" $! (ready δ)).
+    ewp_pure_steps.
+    iLöb as "IH" forall (main q Φ n).
+    iSpecialize ("Hmain" with "[Hℓstate]").
+    { rewrite /fiberContext /fiberState. iExists _. iSplit; first done. by iExists _. }
     iApply (ewp_deep_try_with with "Hmain").
     iLöb as "IH_handler" forall (q Φ).
     iDestruct "Hq" as "#Hq".
     rewrite deep_handler_unfold.
     iSplit; [|iSplit]; last (by iIntros (??) "HFalse"; rewrite upcl_bottom).
     (* Return branch. *)
-    - iIntros (?) "_".
-      ewp_pure_steps. iApply (ewp_next with "HpInv Hq").
+    - iIntros (?) "(_ & HfCtx)".
+      ewp_pure_steps. 
+      by iApply (ewp_next with "HfCtx HpInv Hq").
     (* Effect branch. *)
-    - iIntros (request k). rewrite upcl_Coop upcl_FORK upcl_SUSPEND.
-      iIntros "[(%e & -> & (_ & He) & Hk)
-               |(%suspender & %P & -> & (Hsuspender & _) & Hk)]".
+    - iIntros (request k). rewrite upcl_Coop upcl_FORK upcl_SUSPEND upcl_GET_CONTEXT.
+      iIntros "[(%ℓstate' & %e & -> & (HfState' & He) & Hk)
+               |[(%suspender & %P & -> & (Hsuspender & HfCtx & _) & Hk)
+               |(%_ & -> & _ & Hk)]]".
       (* Fork. *)
-      + ewp_pure_steps.
+      + iDestruct (fiber_state_agree with "HfState' HIsState") as (->) "HfState'".
+        ewp_pure_steps.
         iApply (ewp_bind' (AppRCtx _)); first by done. simpl.
         iApply (ewp_mono with "[Hk]").
         { iApply (queue_push_spec with "Hq"). rewrite /ready.
-          iIntros "#HpInv'". ewp_pure_steps.
-          iSpecialize ("Hk" $! #() with "[//]").
-          iApply "Hk". iNext.
+          iIntros "HfCtx #HpInv'". ewp_pure_steps.
+          iDestruct (fiber_context_agree with "HfCtx HIsState") as "HfState''".
+          iSpecialize ("Hk" $! #() with "HfState''").
+          iApply "Hk". iNext. 
           by iApply ("IH_handler" with "Hq").
         }
         iIntros (?) "_ !>". ewp_pure_steps.
-        iSpecialize ("He" with "HpInv").
-        iApply ("IH" with "[He] Hq").
-        instantiate (1:=(λ _, True)%I).
-        iApply (ewp_mono with "He"). 
-        iIntros (?) "_ !>". by iFrame. 
-      (* Suspend. *)
-      + do 9 ewp_value_or_step.
+        (* find out the current state. a.d. TODO it should be sufficient to just have n existentially quantified
+           in the precondition of IH. *)
+        iDestruct "HfState'" as "(_ & (% & Hℓstate))".
+        iApply ("IH" with "[He] Hℓstate Hq").
+        { instantiate (1:=(λ _, True)%I).
+          iIntros "HfCtx".
+          iSpecialize ("He" with "HfCtx").
+          iApply (ewp_mono with "He"). 
+          iIntros (?) "HfCtx !>". by iFrame. }
+      (* Suspend/GetContext. *)
+      + do 12 ewp_value_or_step.
+        ewp_bind_rule. simpl.
         (* here we bind the creation of waker. Now we should prove a spec for it. *)
         set (Hwaker := (λ (waker: val), (∀ (v : val),
               P v -∗
@@ -926,7 +1067,7 @@ Section verification.
           iIntros (v) "HP".
           ewp_pure_steps.
           iApply (queue_push_spec with "Hq"). rewrite /ready.
-          iIntros "#HpInv'". ewp_pure_steps.
+          iIntros "HfCtx _". ewp_pure_steps.
           iSpecialize ("Hk" $! v with "[$]").
           iApply "Hk". iNext.
           by iApply ("IH_handler" with "Hq").
@@ -937,7 +1078,10 @@ Section verification.
         ewp_bind_rule. simpl.
         iApply (ewp_mono with "Hsuspender").
         iIntros (?) "_ !>". ewp_pure_steps.
-        iApply (ewp_next with "HpInv Hq").
+        iApply (ewp_next with "HfCtx HpInv Hq").
+      + do 12 ewp_value_or_step.
+        iApply ("Hk" with "[$]"). iNext.
+        iApply ("IH_handler" with "Hq").
   Qed.
 
 End verification.
@@ -950,20 +1094,25 @@ Section specification.
   Context `{!ListLib Σ}.
 
   Class AsyncCompLib := {
-    coop : iEff Σ;
+    coop : gname → iEff Σ;
+    is_fiber_state : gname → loc → iProp Σ;
+    fiber_context : gname → iProp Σ;
     is_promise : val → (val -> iProp Σ) → iProp Σ;
     is_promise_Persistent p Φ : Persistent (is_promise p Φ);
     promise_inv : iProp Σ;
-    fork_spec (f : val) Φ :
-      promise_inv ∗ EWP f #() <| coop |> {{ y, □ Φ y }} -∗
-        EWP fork_promise f <| coop |> {{ p, is_promise p Φ }};
-    await_spec p Φ :
-      promise_inv ∗ is_promise p Φ -∗
-        EWP await p <| coop |> {{ y, □ Φ y }};
+    fork_spec δ (f : val) Φ :
+      fiber_context δ ∗ promise_inv ∗ (fiber_context δ -∗ EWP f #() <| coop δ |> {{ y, □ Φ y ∗ fiber_context δ }}) -∗
+        EWP fork_promise f <| coop δ |> {{ p, is_promise p Φ ∗ fiber_context δ }};
+    await_spec δ p Φ :
+      fiber_context δ ∗ promise_inv ∗ is_promise p Φ -∗
+        EWP await p <| coop δ |> {{ y, □ Φ y ∗ fiber_context δ }};
+    get_context_spec δ :
+      ⊢ EWP get_context #() <| coop δ |> {{ state, ∃ (ℓstate: loc), ⌜ state = #ℓstate ⌝ ∗ is_fiber_state δ ℓstate }} ;    
   }.
 
   Definition run_spec (main : val) :=
-    (∀ _ : AsyncCompLib, EWP main #() <| coop |> {{ _, □ True }}) ={⊤}=∗
+    (* a.d. TODO remove the □ True *)
+    (∀ _ : AsyncCompLib, ∀ δ, fiber_context δ -∗ EWP main #() <| coop δ |> {{ _, □ True ∗ fiber_context δ }}) ={⊤}=∗
       EWP run main <| ⊥ |> {{ _, True }}.
 
 End specification.
@@ -994,12 +1143,25 @@ Section closed_proof.
   Local Program Instance async_comp_lib `{!promiseGS Σ} :
     AsyncCompLib (Σ:=Σ) := {
     coop := Coop;
+    is_fiber_state := isFiberState;
+    fiber_context := fiberContext;
     is_promise := λ v Φ, (∃ (p : loc), ⌜ v = #p ⌝ ∗ isPromise p Φ)%I;
     is_promise_Persistent := _;
     promise_inv := promiseInv;
+    get_context_spec := ewp_get_context;
   }.
-  Next Obligation. by iIntros (???) "[??]"; iApply ewp_fork_promise; iFrame. Qed.
-  Next Obligation. by iIntros (???) "(? & % & -> & ?)"; iApply ewp_await; iFrame. Qed.
+  Next Obligation.
+   iIntros (????) "(HfCtx&HpInv&Hf)". 
+   iApply (ewp_mono with "[HfCtx HpInv Hf]").
+   iApply ewp_fork_promise. iFrame.
+   iIntros (?) "(%&->&H2&H3)".
+   iModIntro.
+   iFrame. iExists _. by iFrame.
+  Qed.
+  Next Obligation. 
+    iIntros (????) "(HfCtx & ? & % & -> & ?)". 
+    iApply ewp_await; iFrame. 
+  Qed.
 
   Theorem run_correct main : run_spec main.
   Proof.
@@ -1012,3 +1174,5 @@ Section closed_proof.
     by iAssumption.
   Qed.
 End closed_proof.
+
+Print Assumptions  run_correct.
